Coq/hoare.v
@@ -1,0 +1,1287 @@
+Require Import common.
+Require Import loo_def.
+Require Import loo_properties.
+Require Import loo_reduction_properties.
+Require Import decoupled_classical_properties.
+Require Import decoupling.
+Require Import sbst_decoupled.
+Require Import function_operations.
+Require Import List.
+Require Import CpdtTactics.
+Require Import Coq.Logic.FunctionalExtensionality.
+
+(*Inductive condition : Type :=
+| cond : (config -> Prop) -> condition
+| cond_and : condition -> condition -> condition
+| cond_or : condition -> condition -> condition.
+
+Notation "P '⩟' Q" := (cond_and P Q)(at level 40).
+Notation "P '⊻' Q" := (cond_or P Q)(at level 40).
+
+Fixpoint app (P : condition)(σ : config) :=
+  match goal with
+  | cond Q => Q σ
+  | Q ⩟ R => (app Q σ) /\ (app R σ)
+  | Q ⊻ R => (app Q σ) \/ (app R σ) ∀
+  end.*)
+
+Inductive pair_reductions_alt : mdl -> mdl -> config -> config -> Prop :=
+| pra_single : forall M1 M2 σ1 σ2, M1 ⦂ M2 ⦿ σ1 ⤳ σ2 ->
+                              pair_reductions_alt M1 M2 σ1 σ2
+| pra_trans : forall M1 M2 σ1 σ σ2, M1 ⦂ M2 ⦿ σ1 ⤳ σ ->
+                               pair_reductions_alt M1 M2 σ σ2 ->
+                               pair_reductions_alt M1 M2 σ1 σ2.
+
+Hint Constructors pair_reductions_alt.
+
+Lemma pair_reductions_alt_equiv_1 :
+  forall M1 M2 σ1 σ2, pair_reductions_alt M1 M2 σ1 σ2 ->
+                 M1 ⦂ M2 ⦿ σ1 ⤳⋆ σ2.
+Proof.
+Admitted.
+
+Lemma pair_reductions_alt_equiv_2 :
+  forall M1 M2 σ1 σ2, M1 ⦂ M2 ⦿ σ1 ⤳⋆ σ2 ->
+                 pair_reductions_alt M1 M2 σ1 σ2.
+Proof.
+Admitted.
+
+Lemma pair_reduction_change_alt :
+  forall M1 M2 σ1 σ2, pair_reductions_alt M1 M2 σ1 σ2 ->
+                 forall (P : mdl -> mdl -> config -> Prop),
+                   P M1 M2 σ1 ->
+                   ~ P M1 M2 σ2 ->
+                   exists σ σ', (σ = σ1 \/ pair_reductions_alt M1 M2 σ1 σ) /\
+                           M1 ⦂ M2 ⦿ σ ⤳ σ' /\
+                           (σ' = σ2 \/ pair_reductions_alt M1 M2 σ' σ2) /\
+                           P M1 M2 σ /\
+                           ~ P M1 M2 σ'.
+Proof.
+  intros M1 M2 σ1 σ2 Hred;
+    induction Hred;
+    intros;
+    auto with loo_db.
+
+  - exists σ1, σ2; repeat split;
+      auto.
+
+  - destruct (excluded_middle (P M1 M2 σ)).
+    + specialize (IHHred P);
+        repeat auto_specialize;
+        repeat destruct_exists_loo;
+        andDestruct.
+      exists σ0, σ3; repeat split; eauto.
+      right.
+      destruct Ha;
+        subst;
+        eauto.
+
+    + exists σ1, σ;
+        repeat split;
+        eauto.
+Qed.
+
+Lemma pair_reduction_change :
+  forall M1 M2 σ1 σ2, M1 ⦂ M2 ⦿ σ1 ⤳⋆ σ2 ->
+                 forall (P : mdl -> mdl -> config -> Prop),
+                   P M1 M2 σ1 ->
+                   ~ P M1 M2 σ2 ->
+                   exists σ σ', (σ = σ1 \/ M1 ⦂ M2 ⦿ σ1 ⤳⋆ σ) /\
+                           M1 ⦂ M2 ⦿ σ ⤳ σ' /\
+                           (σ' = σ2 \/ M1 ⦂ M2 ⦿ σ' ⤳⋆ σ2) /\
+                           P M1 M2 σ /\
+                           ~ P M1 M2 σ'.
+Proof.
+  intros.
+  destruct (pair_reduction_change_alt M1 M2 σ1 σ2)
+    with (P:=P)
+    as [σ];
+    auto.
+  apply pair_reductions_alt_equiv_2; auto.
+  repeat destruct_exists_loo;
+    andDestruct.
+  exists σ, σ0;
+    repeat split;
+    auto.
+  + destruct Ha; auto.
+    right; apply pair_reductions_alt_equiv_1; auto.
+  + destruct Ha1; auto.
+    right; apply pair_reductions_alt_equiv_1; auto.
+Qed.
+
+Reserved Notation "M '∙' '{pre:' P '}' σ '{post:' Q '}'" (at level 40).
+Reserved Notation "M '∙' '{pre:' P '}' σ1 '⤳⋆' σ2 '{post:' Q '}'" (at level 40).
+Reserved Notation "M1 '⦂' M2 '⦿' '{pre:' P '}' σ '{post:' Q '}'" (at level 40).
+
+Inductive hoare_triple : mdl -> (config -> Prop) -> config -> (config -> Prop) -> Prop :=
+| ht_r : forall M σ (P Q : config -> Prop), (forall σ', P σ ->
+                                          M ∙ σ ⤳ σ' ->
+                                          Q σ') ->
+                                   M ∙ {pre: P} σ {post: Q}
+
+where "M '∙' '{pre:' P '}' σ '{post:' Q '}'"
+        := (hoare_triple M P σ Q).
+
+Inductive hoare_triples : mdl -> (config -> Prop) -> config -> config -> (config -> Prop) -> Prop :=
+| ht_single : forall M P σ1 σ2 Q, M ∙ σ1 ⤳ σ2 ->
+                             M ∙ {pre: P} σ1 {post: Q} ->
+                             M ∙ {pre: P} σ1 ⤳⋆ σ2 {post: Q}
+| ht_trans : forall M P σ1 σ σ2 P' Q, M ∙ σ1 ⤳ σ ->
+                                 M ∙ {pre: P} σ1 {post: P'} ->
+                                 M ∙ {pre: P'} σ ⤳⋆ σ2 {post: Q} ->
+                                 M ∙ {pre: P} σ1 ⤳⋆ σ2 {post: Q}
+                              
+
+where "M '∙' '{pre:' P '}' σ1 '⤳⋆' σ2 '{post:' Q '}'" := (hoare_triples M P σ1 σ2 Q).
+
+Inductive hoare_triple_pr : mdl -> mdl -> (config -> Prop) -> config -> (config -> Prop) -> Prop :=
+| ht_pr : forall M1 M2 σ (P Q : config -> Prop), (forall σ', P σ ->
+                                               M1 ⦂ M2 ⦿ σ ⤳ σ' ->
+                                               Q σ') ->
+                                        M1 ⦂ M2 ⦿ {pre: P } σ {post: Q }
+
+where "M1 '⦂' M2 '⦿' '{pre:' P '}' σ '{post:' Q '}'"
+        := (hoare_triple_pr M1 M2 P σ Q).
+
+Hint Constructors hoare_triple hoare_triples hoare_triple_pr : loo_db.
+
+Notation "M1 '⦂' M2 '◎' σ0 '…' '⋆' '⊨' '{pre:' A1 '}' σ '{post:' A2 '}'" :=
+  (M1 ⦂ M2 ⦿ {pre: fun σ => M1 ⦂ M2 ◎ σ0 … σ ⊨ A1} σ {post: fun σ' => M1 ⦂ M2 ◎ σ0 … σ' ⊨ A2})(at level 40).
+
+Inductive contn_is : stmt -> config -> Prop :=
+| is_stmt : forall s σ ϕ ψ, snd σ = ϕ :: ψ ->
+                       contn ϕ = c_stmt s ->
+                       contn_is s σ.
+
+Hint Constructors contn_is : loo_db.
+
+Definition is_assgn : config -> Prop :=
+  fun σ => exists r1 r2 s, contn_is (r1 ≔ r2 ;; s) σ.
+
+Definition is_eAssgn : config -> Prop :=
+  fun σ => exists x e s, contn_is (x ≔′ e ;; s) σ.
+
+Definition is_fAccess : config -> Prop :=
+  fun σ => exists x y f s, contn_is (r_ x ≔ (y ◌ f) ;; s) σ.
+
+Definition is_fAssgn : config -> Prop :=
+  fun σ => exists x f y s, contn_is (x ◌ f ≔ (r_ y) ;; s) σ.
+
+Definition is_new : config -> Prop :=
+  fun σ => exists x C β s, contn_is (s_new x C β ;; s) σ.
+
+Definition is_if : config -> Prop :=
+  fun σ => exists e s1 s2 s, contn_is (s_if e s1 s2 ;; s) σ.
+
+Definition is_rtrn : config -> Prop :=
+  fun σ => exists x, (contn_is (s_rtrn x) σ \/
+              exists s, contn_is (s_rtrn x ;; s) σ).
+
+(*Definition is_reduced : config -> config -> Prop :=
+  fun σ1 σ2 => exists ϕ1 ϕ2 ψ s1 s2, snd σ1 = ϕ1 :: ψ /\
+                             snd σ2 = ϕ2 :: ψ /\
+                             contn ϕ1 = c_stmt (s1 ;; s2) /\
+                             contn ϕ2 = c_stmt s2.*)
+
+Definition ctxUpdated : config -> var -> value -> config -> Prop :=
+  fun σ1 x v σ2 => exists ϕ1 ϕ2 ψ, snd σ1 = ϕ1 :: ψ /\
+                           snd σ2 = ϕ2 :: ψ /\
+                           vMap ϕ2 = update x v (vMap ϕ1).
+
+Definition heapUpdated : config -> addr -> obj -> config -> Prop :=
+  fun σ1 α o σ2 => fst σ2 = (update α o (fst σ1)).
+
+Definition fieldHeapUpdated : config -> addr -> fld -> value -> config -> Prop :=
+  fun σ1 α f v σ2 => exists o' v', ⟦ α ↦ o' ⟧ ∈ σ1 /\
+                           flds o' f = Some v' /\
+                           heapUpdated σ1 α (new (cname o') (update f v (flds o'))) σ2.
+
+Definition fieldUpdated : config -> var -> fld -> var -> config -> Prop :=
+  fun σ1 x f y σ2 => exists α v, ⌊ x ⌋ σ1 ≜ (v_addr α) /\
+                         ⌊ y ⌋ σ2 ≜ v /\
+                         fieldHeapUpdated σ1 α f v σ2.
+
+Definition fieldMapsTo : config -> var -> fld -> value -> Prop :=
+  fun σ x f v => exists α o, ⌊ x ⌋ σ ≜ (v_addr α) /\
+                     ⟦ α ↦ o ⟧ ∈ σ /\
+                     flds o f = Some v.
+
+Definition new_object_created : config -> var -> cls -> partial_map fld var -> config -> Prop :=
+  fun σ x C ps σ' =>  exists χ ϕ ψ α s, σ = (χ, ϕ :: ψ) /\
+                                contn ϕ = c_stmt (s_new x C ps ;; s) /\
+                                fresh_χ χ α /\
+                                heapUpdated σ α (new C (ps ∘ (vMap ϕ))) σ' /\
+                                ctxUpdated σ x (v_addr α) σ'.
+
+Definition heapUnchanged : config -> config -> Prop :=
+  fun σ1 σ2 => fst σ1 = fst σ2.
+
+Definition ctxUnchanged : config -> config -> Prop :=
+  fun σ1 σ2 => exists ϕ1 ϕ2 ψ, snd σ1 = ϕ1 :: ψ /\
+                       snd σ2 = ϕ2 :: ψ /\
+                       vMap ϕ1 = vMap ϕ2.
+
+Ltac hoare_auto :=
+  intros;
+  repeat destruct_exists_loo;
+  unfold is_eAssgn in *;
+  unfold is_fAccess in *;
+  unfold is_fAssgn in *;
+  unfold is_if in *;
+  unfold is_new in *;
+  unfold heapUnchanged in *; simpl in *;
+  andDestruct;
+  simpl in *;
+  subst;
+  match goal with
+  | [ |- _ ∙ {pre: _} _ {post: _}] =>
+    apply ht_r;
+    intros
+  | [Hcontn : contn_is _ _ |- _] =>
+    inversion Hcontn;
+    subst;
+    clear Hcontn
+  | [|- contn_is _ (_, ?ϕ' :: ?ψ')] =>
+    eapply is_stmt with (ϕ:=ϕ')(ψ:=ψ');
+    eauto
+  | [Hred : _ ∙ _ ⤳ _ |- _] =>
+    inversion Hred;
+    subst;
+    clear Hred;
+    repeat simpl_crush
+  end;
+  try solve [repeat (eexists; simpl in *); eauto];
+             repeat (destruct_exists_loo; andDestruct).
+
+Lemma eAssgn_hoare :
+  forall M σ x e s, M ∙ {pre: contn_is (x ≔′ e ;; s)} σ {post: fun σ' => (contn_is s σ') /\
+                                                                 (exists v, ctxUpdated σ x v σ' /\
+                                                                       M ∙ σ ⊢ e ↪ v)}.
+Proof.
+  intros M σ;
+    destruct σ as [χ ψ];
+    repeat hoare_auto.
+Qed.
+
+Lemma eAssgn_heap_unchanged_hoare :
+  forall M σ x e s, M ∙ {pre: contn_is (x ≔′ e ;; s)} σ {post: heapUnchanged σ}.
+Proof.
+  intros M σ;
+    destruct σ as [χ ψ];
+    repeat hoare_auto.
+Qed.
+
+Lemma fAccess_hoare :
+  forall M σ x y f s, M ∙
+                   {pre: contn_is (r_ x ≔ (y ◌ f) ;; s)}
+                   σ
+                   {post: fun σ' => contn_is s σ' /\
+                                 (exists v, fieldMapsTo σ y f v /\
+                                       ctxUpdated σ x v σ')}.
+Proof.
+  intros M σ;
+    destruct σ as [χ ψ];
+    repeat hoare_auto.
+
+  repeat eexists; eauto.
+
+  match goal with
+    [Hint : ⌊ _ ⌋ _ ≜ _ |- _] =>
+    inversion Hint;
+      subst
+  end;
+    simpl in *;
+    repeat simpl_crush;
+    auto.
+  
+Qed.
+
+Lemma fAccess_heap_unchanged_hoare :
+  forall M σ x y f s, M ∙
+                   {pre: contn_is (r_ x ≔ (y ◌ f) ;; s)}
+                   σ
+                   {post: heapUnchanged σ}.
+Proof.
+  intros M σ;
+    destruct σ as [χ ψ];
+    repeat hoare_auto.
+Qed.
+
+Lemma fAssgn_hoare :
+  forall M σ x f y s, M ∙
+                   {pre: contn_is (x ◌ f ≔ (r_ y) ;; s)}
+                   σ
+                   {post: fun σ' => contn_is s σ' /\
+                                 fieldUpdated σ x f y σ'}.
+Proof.
+  intros M σ;
+    destruct σ as [χ ψ];
+    repeat hoare_auto.
+  split;
+    try hoare_auto.
+
+  repeat eexists; eauto;
+    try solve [repeat match goal with
+                        [Hint : ⌊ _ ⌋ _ ≜ _ |- _] =>
+                        inversion Hint;
+                        subst;
+                        clear Hint
+                      end;
+               simpl in *;
+               repeat simpl_crush;
+               auto].
+Qed.
+
+Lemma fAssgn_ctx_unchanged_hoare :
+  forall M σ x f y s, M ∙
+                   {pre: contn_is (x ◌ f ≔ (r_ y) ;; s)}
+                   σ
+                   {post: ctxUnchanged σ}.
+Proof.
+  intros M σ;
+    destruct σ as [χ ψ];
+    repeat hoare_auto.
+Qed.
+
+Lemma new_hoare :
+  forall M σ x C β s, M ∙
+                   {pre: contn_is (s_new x C β ;; s)}
+                   σ
+                   {post: fun σ' => contn_is s σ' /\
+                                 new_object_created σ x C β σ'}.
+Proof.
+  intros M σ;
+    destruct σ as [χ ψ];
+    repeat hoare_auto;
+    split;
+    try solve [repeat (eexists; eauto);
+               eauto].
+Qed.
+
+Lemma if_true_hoare :
+  forall M σ e s1 s2 s, M ∙ {pre: fun σ => contn_is (s_if e s1 s2 ;; s) σ /\
+                                   M ∙ σ ⊢ e ↪ v_true}
+                     σ
+                     {post: contn_is (merge s1 s)}.
+Proof.
+  intros M σ;
+    destruct σ as [χ ψ];
+    intros.
+  repeat hoare_auto.
+  eval_rewrite; crush.
+Qed.
+
+Lemma if_false_hoare :
+  forall M σ e s1 s2 s, M ∙ {pre: fun σ => contn_is (s_if e s1 s2 ;; s) σ /\
+                                   M ∙ σ ⊢ e ↪ v_false}
+                     σ
+                     {post: contn_is (merge s2 s)}.
+Proof.
+  intros M σ;
+    destruct σ as [χ ψ];
+    intros.
+  repeat hoare_auto.
+  eval_rewrite; crush.
+Qed.
+
+Lemma if_heap_unchanged_hoare :
+  forall M σ, M ∙ {pre: is_if} σ {post: heapUnchanged σ}.
+Proof.
+  intros M σ;
+    destruct σ as [χ ψ];
+    intros.
+  repeat hoare_auto.
+Qed.
+
+Lemma if_ctx_unchanged_hoare :
+  forall M σ, M ∙ {pre: is_if} σ {post: ctxUnchanged σ}.
+Proof.
+  intros M σ;
+    destruct σ;
+    repeat hoare_auto.
+Qed.
+
+Lemma hoare_triple_inversion :
+  forall M P σ Q, M ∙ {pre: P} σ {post: Q} ->
+             forall σ', M ∙ σ ⤳ σ' ->
+                   P σ -> Q σ'.
+Proof.
+  intros M P σ Q Hhoare;
+    inversion Hhoare;
+    eauto.
+Qed.
+
+Ltac hoare_inversion_1 :=
+  match goal with
+  | [Hhoare : ?M ∙ {pre: ?P} ?σ {post: ?Q},
+              Hred : ?M ∙ ?σ ⤳ ?σ' |- _ ] =>
+    notHyp (Q σ');
+    assert (Q σ');
+    [eapply hoare_triple_inversion; eauto|]
+  end.
+
+Lemma hoare_triples_inversion :
+  forall M P σ1 σ2 Q, M ∙ {pre: P} σ1 ⤳⋆ σ2 {post: Q} ->
+                 P σ1 -> Q σ2.
+Proof.
+  intros M P σ1 σ2 Q Hhoare;
+    induction Hhoare;
+    intros;
+    eauto with loo_db;
+    hoare_inversion_1; eauto.
+Qed.
+
+Ltac hoare_inversion_2 :=
+  match goal with
+  | [Hhoare : ?M ∙ {pre: ?P} ?σ {post: ?Q},
+              Hred : ?M ∙ ?σ ⤳⋆ ?σ' |- _ ] =>
+    notHyp (Q σ');
+    assert (Q σ');
+    [eapply hoare_triples_inversion; eauto|]
+  end.
+
+Lemma hoare_triple_pr_inversion :
+  forall M1 M2 P σ Q, M1 ⦂ M2 ⦿ {pre: P} σ {post: Q} ->
+                 forall σ', M1 ⦂ M2 ⦿ σ ⤳ σ' ->
+                       P σ -> Q σ'.
+Proof.
+  intros M1 M2 P σ Q Hhoare;
+    inversion Hhoare;
+    subst;
+    intros;
+    eauto.
+Qed.
+
+Lemma hoare_triples_pr_transitive :
+  forall M P σ1 σ2 Q, M ∙ {pre: P} σ1 ⤳⋆ σ2 {post: Q} ->
+                 forall σ3 Q', M ∙ {pre: Q} σ2 ⤳⋆ σ3 {post: Q'} ->
+                          M ∙ {pre: P} σ1 ⤳⋆ σ3 {post: Q'}.
+Proof.
+  intros M P σ1 σ2 Q Hhoare;
+    induction Hhoare;
+    intros;
+    simpl;
+    eauto;
+    eapply ht_trans; eauto.
+Qed.
+
+Ltac hoare_inversion :=
+  match goal with
+  | [Hhoare : ?M ∙ {pre: ?P} ?σ {post: ?Q},
+              Hred : ?M ∙ ?σ ⤳ ?σ' |- _ ] =>
+    notHyp (Q σ');
+    assert (Q σ');
+    [eapply hoare_triple_inversion; eauto|]
+  | [Hhoare : ?M ∙ {pre: ?P} ?σ ⤳⋆ ?σ' {post: ?Q} |- _ ] =>
+    notHyp (Q σ');
+    assert (Q σ');
+    [eapply hoare_triples_inversion; eauto|]
+  | [Hhoare : ?M1 ⦂ ?M2 ⦿ {pre: ?P} ?σ {post: ?Q},
+              Hred : ?M1 ⦂ ?M2 ⦿ ?σ ⤳ ?σ' |- _ ] =>
+    notHyp (Q σ');
+    assert (Q σ');
+    [eapply hoare_triple_pr_inversion; eauto|]
+  end.
+
+Lemma reduction_trace_unique :
+  forall M σ1 σ2, M ∙ σ1 ⤳⋆ σ2 ->
+             forall σ3, M ∙ σ1 ⤳⋆ σ3 ->
+                   (M ∙ σ2 ⤳⋆ σ3) \/
+                   (σ2 = σ3) \/
+                   (M ∙ σ3 ⤳⋆ σ2).
+Proof.
+  intros M σ1 σ2 Hred;
+    induction Hred;
+    intros σ Hred';
+    subst.
+
+  - inversion Hred';
+      unique_reduction_auto;
+      eauto.
+
+  - inversion Hred';
+      subst;
+      unique_reduction_auto;
+      eauto.
+Qed.
+
+Lemma reductions_transitive :
+  forall M σ1 σ2, M ∙ σ1 ⤳⋆ σ2 ->
+             forall σ3, M ∙ σ2 ⤳⋆ σ3 ->
+                   M ∙ σ1 ⤳⋆ σ3.
+Proof.
+  intros M σ1 σ2 Hred;
+    induction Hred;
+    intros;
+    eauto with loo_db.
+Qed.
+
+Hint Resolve reductions_transitive : loo_db.
+Hint Rewrite reductions_transitive : loo_db.
+
+Lemma internal_reductions_is_reducions :
+  forall M1 M2 σ1 σ2, M1 ⦂ M2 ⦿ σ1 ⤳… σ2 ->
+                 forall M, M1 ⋄ M2 ≜ M ->
+                      M ∙ σ1 ⤳⋆ σ2.
+Proof.
+  intros M1 M2 σ1 σ2 Hred;
+    induction Hred;
+    intros;
+    link_unique_auto;
+    auto with loo_db.
+
+  - specialize (IHHred M);
+      auto_specialize.
+    eauto with loo_db.
+Qed.
+
+Lemma pair_reduction_is_reductions :
+  forall M1 M2 σ1 σ2, M1 ⦂ M2 ⦿ σ1 ⤳ σ2 ->
+                 forall M, M1 ⋄ M2 ≜ M ->
+                      M ∙ σ1 ⤳⋆ σ2.
+Proof.
+  intros M1 M2 σ1 σ2 Hred;
+    induction Hred;
+    intros;
+    link_unique_auto;
+    auto with loo_db.
+
+  - match goal with
+    | [H : _ ⦂ _ ⦿ _ ⤳… _ |- _] =>
+      eapply internal_reductions_is_reducions in H;
+        eauto with loo_db
+    end.
+Qed.
+
+(**
+reduction_order is an ordering on stacks. 
+This is used to prove that reduction is acyclic.
+reducion_order is not well-founded, as loo has
+recursive functions, and thus a loo program might 
+never terminate. It is only useful as an ordering 
+on stacks to prove reduction acyclic from the 
+perspective of stacks
+
+ro extends this ordering on configurations.
+
+ro σ1 σ2
+
+means σ2 < σ1
+ *)
+
+Definition stmt_of (ϕ : frame) :=
+  match contn ϕ with
+  | c_stmt s => s
+  | c_hole _ s => s
+  end.
+
+Definition contn_size :=
+  fun c => match c with
+        | c_stmt s => stmt_size s
+        | c_hole _ s => 1 + stmt_size s
+        end.
+
+Inductive reduction_order : stack -> stack -> Prop :=
+| ro_frame : forall ψ1 ψ2 ϕ1 ϕ2 ψ, contn_size (contn ϕ1) > contn_size (contn ϕ2) ->
+                              reduction_order (ψ1 ++ ϕ1 :: ψ) (ψ2 ++ ϕ2 :: ψ).
+Hint Constructors reduction_order : loo_db.
+
+Definition ro (σ1 σ2 : config) :=
+  reduction_order (snd σ1) (snd σ2).
+
+Lemma reduction_order_transitive :
+  forall ψ1 ψ2, reduction_order ψ1 ψ2 ->
+           forall ψ3, reduction_order ψ2 ψ3 ->
+                 reduction_order ψ1 ψ3.
+Proof.
+(**
+This is fairly straight-forward to prove on paper.
+By inversion on the derivation of reduction_order, 
+we get:
+
+ψ1 = ψ1' ++ ϕ1 :: ψa
+ψ2 = ψ2_1 ++ ϕ2 :: ψa
+
+and 
+
+ψ2 = ψ2_2 ++ ϕ2' :: ψb
+ψ3 = ψ3' ++ ϕ3 :: ψb
+
+Since 
+
+ψ2_1 ++ ϕ2 :: ψa = ψ2_2 ++ ϕ2' :: ψb, 
+
+it follows that either
+(i) ψa = ψb, (ii) ψa ⊂ ψb, or (iii) ψb ⊂ ψa
+
+(i) derived simply by noting that 
+ϕ2' = ϕ2 and
+contn_size ϕ1 > contn_size ϕ2 > contn_size ϕ3
+
+(ii) it follows that ∃ ψ3'', ψ3 = ψ3'' ++ ϕ2 :: ψa. 
+the desired result follows from this
+
+(iii) it follows that ∃ ψ1'', ψ1 = ψ1'' ++ ϕ2' :: ψb. 
+the desired result follows from this
+*)
+Admitted.
+
+Lemma reduction_is_ordered :
+  forall M σ1 σ2, M ∙ σ1 ⤳ σ2 ->
+             ro σ1 σ2.
+Proof.
+  intros M σ1 σ2 Hred;
+    inversion Hred;
+    subst;
+    unfold ro;
+    simpl in *;
+    try solve [match goal with
+               | [|- reduction_order (?ϕ1 :: ?ψ) (?ϕ2 :: ?ψ)] =>
+                 let Ha := fresh in
+                 let Hb := fresh in
+                 assert (Ha : (ϕ1 :: ψ) = (nil ++ (ϕ1 :: ψ)));
+                 [crush|rewrite Ha];
+                 assert (Hb : (ϕ2 :: ψ) = (nil ++ (ϕ2 :: ψ)));
+                 [crush|rewrite Hb];
+                 apply ro_frame;
+                 simpl
+               end;
+               match goal with
+               | [H : contn ?ϕ = _ |- context[contn ?ϕ]] =>
+                 rewrite H;
+                 simpl
+               end;
+               simpl;
+               try rewrite merge_stmt_size;
+               crush];
+    try solve [match goal with
+               | [|- reduction_order (?ϕ1 :: ?ϕ2 :: ?ψ) (?ϕ :: ?ψ)] =>
+                 let Ha := fresh in
+                 let Hb := fresh in
+                 assert (Ha : (ϕ :: ψ) = (nil ++ (ϕ :: ψ)));
+                 [crush|rewrite Ha];
+                 assert (Hb : (ϕ1 :: ϕ2 :: ψ) = ((ϕ1 :: nil) ++ (ϕ2 :: ψ)));
+                 [crush|rewrite Hb];
+                 apply ro_frame;
+                 simpl
+               end;
+               match goal with
+               | [H : contn ?ϕ = _ |- context[contn ?ϕ]] =>
+                 rewrite H;
+                 simpl
+               end;
+               auto].
+
+  - match goal with
+    | [|- reduction_order (?ϕ :: ?ψ) (?ϕ1 :: ?ϕ2 :: ?ψ)] =>
+      let Ha := fresh in
+      let Hb := fresh in
+      assert (Ha : (ϕ :: ψ) = (nil ++ (ϕ :: ψ)));
+        [crush|rewrite Ha];
+        assert (Hb : (ϕ1 :: ϕ2 :: ψ) = ((ϕ1 :: nil) ++ (ϕ2 :: ψ)));
+        [crush|rewrite Hb];
+        apply ro_frame;
+        simpl
+    end.
+    match goal with
+    | [H : contn ?ϕ = _ |- context[contn ?ϕ]] =>
+      rewrite H;
+        simpl
+    end;
+      auto.
+Qed.
+
+Lemma reductions_is_ordered :
+  forall M σ1 σ2, M ∙ σ1 ⤳⋆ σ2 ->
+             ro σ1 σ2.
+Proof.
+  intros M σ1 σ2 Hred;
+    induction Hred.
+
+  - eapply reduction_is_ordered; eauto.
+
+  - apply reduction_order_transitive with (ψ2:=snd σ2); auto.
+    eapply reduction_is_ordered; eauto.
+Qed.
+
+Lemma reduction_order_implies_neq :
+  forall ψ1 ψ2, reduction_order ψ1 ψ2 ->
+           ψ1 <> ψ2.
+Proof.
+  intros ψ1 ψ2 Hord;
+    inversion Hord;
+    subst.
+Admitted.
+
+Lemma ro_implies_neq :
+  forall σ1 σ2, ro σ1 σ2 ->
+           σ1 <> σ2.
+Proof.
+  intros.
+  apply reduction_order_implies_neq in H.
+  intros Hcontra;
+    subst;
+    crush.
+Qed.
+
+Lemma acyclic_reductions :
+  forall M σ1 σ2, M ∙ σ1 ⤳⋆ σ2 ->
+             σ1 <> σ2.
+Proof.
+  intros.
+  apply ro_implies_neq.
+  eapply reductions_is_ordered; eauto.
+Qed.
+
+(*Lemma internal_reductions_are_internal :
+  forall M1 M2 σ1 σ2, M1 ⦂ M2 ⦿ σ1 ⤳… σ2 ->
+                 forall M σ, M1 ⋄ M2 ≜ M ->
+                        M ∙ σ1 ⤳⋆ σ ->
+                        M ∙ σ ⤳⋆ σ2 ->
+                        internal_self M1 M2 σ.
+Proof.
+  intros M1 M2 σ1 σ2 Hred;
+    induction Hred;
+    intros;
+    link_unique_auto.
+
+  - 
+
+Qed.*)
+
+Lemma hoare_reductions_implies_pair_reduction :
+  forall M P σ1 σ2 Q, M ∙ {pre: P} σ1 ⤳⋆ σ2 {post: Q} ->
+                 forall M1 M2, M1 ⋄ M2 ≜ M ->
+                          M1 ⦂ M2 ⦿ σ1 ⤳ σ2 ->
+                          M1 ⦂ M2 ⦿ {pre: P} σ1 {post: Q}.
+Proof.
+  intros M P σ1 σ2 Q Hhoare;
+    intros.
+
+  apply ht_pr; intros.
+  unique_reduction_auto.
+  match goal with
+  | [H : _ ⦂ _ ⦿ _ ⤳ _ |- _] =>
+    eapply pair_reduction_is_reductions in H;
+      eauto
+  end.
+  hoare_inversion; auto.
+Qed.
+
+Definition empty_precondition := (fun (_ : config) => True).
+Notation "∅" := (empty_precondition)(at level 40).
+
+Definition waiting_frame_is :=
+  fun (f : config -> Prop) σ => exists ϕ1 ϕ2 ψ, snd σ = ϕ1 :: ϕ2 :: ψ /\
+                                    f (fst σ, ϕ2 :: ψ).
+
+Definition is_return_to :=
+  fun (f : config -> Prop) σ => is_rtrn σ /\
+                         waiting_frame_is f σ.
+
+Definition is_call_to :=
+  fun (f : config -> var -> Prop) σ => exists x y m β s, contn_is (s_meth x y m β ;; s) σ /\
+                                            f σ y.
+
+Definition external_step :=
+  fun (M1 M2 : mdl) σ => external_self M1 M2 σ /\
+                      (is_assgn σ \/
+                       is_new σ \/
+                       is_if σ \/
+                       is_call_to (is_external M1 M2) σ \/
+                       is_return_to (external_self M1 M2) σ).
+
+Definition internal_step :=
+  fun M1 M2 σ => is_call_to (is_internal M1 M2) σ \/
+              is_return_to (internal_self M1 M2) σ.
+
+Lemma internal_self_update_contn :
+  forall M1 M2 σ, internal_self M1 M2 σ ->
+             forall c, internal_self M1 M2 (update_σ_contn σ c).
+Proof.
+  intros M1 M2 σ Hinternal c.
+  destruct σ as [χ ψ].
+  unfold update_σ_contn; simpl.
+  destruct ψ as [|ϕ ψ];
+    [crush|].
+  eauto.
+Qed.
+
+Lemma internal_self_update_vMap :
+  forall M1 M2 σ, internal_self M1 M2 σ ->
+             forall x v, x <> this -> internal_self M1 M2 (update_σ_map σ x v).
+Proof.
+  intros M1 M2 σ Hinternal x v Hneq.
+  destruct σ as [χ ψ].
+  destruct ψ as [|ϕ ψ];
+    [crush|].
+  repeat map_rewrite.
+  unfold update_ϕ_map.
+  unfold internal_self, is_internal in *.
+  repeat destruct_exists_loo;
+    andDestruct.
+  repeat eexists;
+    simpl;
+    eauto.
+  repeat map_rewrite.
+  unfold vMap.
+  eq_auto.
+Qed.
+
+Lemma internal_step_is_internal :
+  forall M σ1 σ2, M ∙ σ1 ⤳ σ2 ->
+             forall M1 M2, M1 ⋄ M2 ≜ M ->
+                      internal_step M1 M2 σ1 ->
+                      internal_self M1 M2 σ2.
+Proof.
+  intros M σ1 σ2 Hred;
+    inversion Hred;
+    intros;
+    subst;
+    try solve [unfold internal_step in *;
+               match goal with
+               | [H : is_call_to _ _ \/ is_return_to _ _ |- _] =>
+                 let H' := fresh in
+                 destruct H as [H'|H']
+               end;
+               unfold is_call_to, is_return_to, is_rtrn in *;
+               repeat destruct_exists_loo;
+               andDestruct;
+               repeat destruct_exists_loo;
+               try match goal with
+                   | [H : contn_is _ _ \/ _ |- _] =>
+                     destruct H
+                   end;
+               repeat destruct_exists_loo;
+               try match goal with
+                   | [Ha : contn_is _ ?ϕ |- _] =>
+                     inversion Ha;
+                     subst;
+                     simpl in *
+                   end;
+               repeat simpl_crush];
+    try solve [unfold internal_step in *;
+               match goal with
+               | [H : is_call_to _ _ \/ is_return_to _ _ |- _] =>
+                 let H' := fresh in
+                 destruct H as [H'|H']
+               end;
+               unfold is_call_to, is_return_to, is_rtrn in *;
+               repeat destruct_exists_loo;
+               andDestruct;
+               repeat destruct_exists_loo;
+               try match goal with
+                   | [H : contn_is _ _ \/ _ |- _] =>
+                     destruct H
+                   end;
+               repeat destruct_exists_loo;
+               try match goal with
+                   | [Ha : contn_is _ ?ϕ |- _] =>
+                     inversion Ha;
+                     subst;
+                     simpl in *
+                   end;
+               repeat simpl_crush;
+               unfold waiting_frame_is in *;
+               repeat destruct_exists_loo;
+               andDestruct;
+               simpl in *;
+               repeat simpl_crush;
+               assert (Htmp : (χ, update_ϕ_contn (update_ϕ_map ϕ1 y α) (c_stmt s) :: ψ0) =
+                              (update_σ_contn (update_σ_map (χ, ϕ1 :: ψ0) y α) (c_stmt s)));
+               [auto|rewrite Htmp];
+               apply internal_self_update_contn, internal_self_update_vMap; auto].
+
+  - match goal with
+    | [H : internal_step ?M1 ?M2 (?χ, ?ϕ :: ?ψ) |- _] =>
+      let Ha := fresh in
+      unfold internal_step in H;
+        destruct H as [Ha|Ha];
+        unfold is_call_to, is_return_to in Ha;
+        repeat destruct_exists_loo;
+        andDestruct
+    end.
+    + match goal with
+      | [H : contn_is _ _ |- _] =>
+        inversion H;
+          subst;
+          simpl in *
+      end.
+      repeat simpl_crush.
+
+      
+      unfold is_internal in Hb;
+        repeat destruct_exists_loo;
+        andDestruct;
+        repeat simpl_crush.
+      inversion H2; subst;
+        simpl in *;
+        repeat simpl_crush.
+      repeat map_rewrite.
+      repeat simpl_crush.
+      unfold internal_self, is_internal;
+        repeat map_rewrite;
+        simpl;
+        repeat eexists;
+        eauto.
+
+    + match goal with
+      | [H : is_rtrn _ |- _] =>
+        let H' := fresh in
+        let x := fresh "x" in
+        unfold is_rtrn in H;
+          destruct H as [x H'];
+          destruct H';
+          repeat destruct_exists_loo;
+          try match goal with
+              | [Ha : contn_is _ ?ϕ |- _] =>
+                inversion Ha;
+                  subst;
+                  simpl in *
+              end;
+          repeat simpl_crush
+      end.
+
+Qed.
+
+Lemma internal_reductions_is_internal_step :
+  forall M1 M2 σ1 σ2, M1 ⦂ M2 ⦿ σ1 ⤳… σ2 ->
+                 internal_step M1 M2 σ1.
+Proof.
+  intros M1 M2 σ1 σ2 Hred;
+    induction Hred;
+    intros; auto.
+
+  unfold internal_step.
+
+  match goal with
+  | [H : _ ∙ _ ⤳ _ |- _] =>
+    inversion H; subst;
+      eauto
+  end.
+
+  - admit.
+
+   
+Admitted.
+
+Lemma external_self_implies_external_step :
+  forall M σ1 σ2, M ∙ σ1 ⤳ σ2 ->
+             forall M1 M2, M1 ⋄ M2 ≜ M ->
+                      external_self M1 M2 σ2 ->
+                      external_step M1 M2 σ1.
+Proof.
+
+Admitted.
+
+Lemma pair_reduction_inversion_hoare :
+  forall M1 M2 σ1 σ2, M1 ⦂ M2 ⦿ σ1 ⤳ σ2 ->
+                 external_step M1 M2 σ1 \/
+                 internal_step M1 M2 σ1.
+Proof.
+  intros M1 M2 σ1 σ2 Hred;
+    induction Hred;
+    intros.
+
+  - right; eapply internal_reductions_is_internal_step; eauto.
+
+  - left; eapply external_self_implies_external_step; eauto.
+
+Qed.
+
+Lemma external_step_leaves_internal_unchanged :
+  forall M1 M2 σ, external_step M1 M2 σ ->
+             forall σ0 α o, M1 ⦂ M2 ⦿
+                          {pre: fun σ => ⟦ α ↦ o ⟧ ∈ σ /\
+                                      M1 ⦂ M2 ◎ σ0 … σ ⊨ ((a_ α) internal)}
+                          σ
+                          {post: fun σ' => ⟦ α ↦ o ⟧ ∈ σ'}.
+Proof.
+Admitted.
+
+Lemma fieldChange_not_heapUnchanged :
+  forall M1 M2 σ0 σ α f v, M1 ⦂ M2 ◎ σ0 … ⋆ ⊨ {pre: ex_acc_f (e_ α) f ⩶̸ v} σ {post: ex_acc_f (e_ α) f ⩶ v} ->
+                      forall σ', M1 ⦂ M2 ⦿ σ ⤳ σ' ->
+                            ~ heapUnchanged σ σ'.
+Proof.
+
+Admitted.
+
+Lemma not_eq_implies_neq :
+  forall M1 M2 σ0 σ e1 e2, ~ M1 ⦂ M2 ◎ σ0 … σ ⊨ (e1 ⩶ e2) ->
+                      M1 ⦂ M2 ◎ σ0 … σ ⊨ (e1 ⩶̸ e2).
+Proof.
+Admitted.
+
+Lemma not_neq_implies_eq :
+  forall M1 M2 σ0 σ e1 e2, ~ M1 ⦂ M2 ◎ σ0 … σ ⊨ (e1 ⩶̸ e2) ->
+                      M1 ⦂ M2 ◎ σ0 … σ ⊨ (e1 ⩶ e2).
+Proof.
+Admitted.
+
+Lemma external_step_leaves_internal_field_unchanged :
+  forall M1 M2 σ0 σ α, M1 ⦂ M2 ◎ σ0 … σ ⊨ ((a_ α) internal) ->
+                  forall f v, M1 ⦂ M2 ◎ σ0 … σ ⊨ (ex_acc_f (e_ α) f ⩶̸ v) ->
+                         external_step M1 M2 σ ->
+                         forall σ', M1 ⦂ M2 ⦿ σ ⤳ σ' ->
+                               M1 ⦂ M2 ◎ σ0 … σ' ⊨ (ex_acc_f (e_ α) f ⩶̸ v).
+Proof.
+
+Admitted.
+
+Lemma internal_class_implies_internal :
+  forall M1 M2 σ0 σ α C, M1 ⦂ M2 ◎ σ0 … σ ⊨ (a_class (a_ α) C) ->
+                    (exists CDef, M1 C = Some CDef) ->
+                    forall σ0' σ', M1 ⦂ M2 ◎ σ0' … σ' ⊨ ((a_ α) internal).
+Proof.
+Admitted.
+
+Module SafeExample.
+
+  (**
+∀s.[s : Safe ∧ s.treasure <> null ∧ will(s.treasure = null) 
+        ⟶ ∃o.[external(o) ∧ (o access s.secret)]]
+   *)
+
+  (** Safe Definition *)
+
+  Definition Safe := classID 1.
+
+  Definition treasure := fieldID 0.
+
+  Definition secret := fieldID 1.
+
+  Definition take := methID 0.
+
+  Definition scr := bnd 1.
+
+  Definition x := bnd 2.
+
+  Definition y := bnd 3.
+
+  Definition takeBody := ((r_ x) ≔ (r_exp (e_val (v_null)))) ;;
+                         (((r_ y) ≔ (this ◌ treasure)) ;;
+                          ((s_if ((e_var scr) ⩵ (e_acc_f (e_var this) secret))
+                                 (((this ◌ treasure) ≔ (r_ x)) ;;
+                                  (s_rtrn y))
+                                 (s_rtrn x)) ;;
+                           (s_rtrn x))).
+
+  Definition SafeDef1 := clazz Safe
+                               (treasure :: secret :: nil)
+                               (update
+                                  take (scr :: nil, takeBody)
+                                  empty)
+                               empty.
+
+
+  (**
+σ ⊨ o ∈ Provides (S) iff
+            ∃ σ’.
+                [ σ ⤳^* σ’ &&
+                  ∃ o’: [ σ ⊨ External<o’> && σ ⊨ ¬ Access<o’,o>
+                                  &&  σ’ ⊨  Access<o,o’> ]
+                 ]
+
+*)
+
+  (** MyModule Definition *)
+
+  Definition MyModule1 := (update
+                             Safe SafeDef1
+                             empty).
+
+  Lemma link_MyModule1_Safe :
+    forall M' M, MyModule1 ⋄ M' ≜ M ->
+            M Safe = Some SafeDef1.
+  Proof.
+    intros.
+    inversion H;
+      subst;
+      simpl.
+    unfold MyModule1, extend in *; simpl.
+    repeat map_rewrite.
+  Qed.
+
+  Ltac pr_linking :=
+    match goal with
+    | [Hred : ?Ma ⦂ ?Mb ⦿ ?σ ⤳ ?σ' |- _ ] =>
+      let H := fresh in
+      let M := fresh "M'" in
+      assert (H : exists M', Ma ⋄ Mb ≜ M');
+      [inversion Hred; eauto|destruct H as [M']]
+      
+    end.
+
+  Ltac hoare_pair_reduction_step :=
+    match goal with
+    | [|- ?Ma ⦂ ?Mb ⦿ {pre: ?P} ?σa {post: ?Q}] =>
+      destruct (excluded_middle (exists σ', Ma ⦂ Mb ⦿ σa ⤳ σ')) as [|Hcontra];
+      [destruct_exists_loo
+      |apply ht_pr;
+       intros;
+       contradiction Hcontra;
+       eauto;
+       apply hoare_reductions_implies_pair_reduction];
+      pr_linking;
+      try link_unique_auto;
+      match goal with
+      | [Hlink : Ma ⋄ Mb ≜ ?Mc,
+                 Hred : Ma ⦂ Mb ⦿ σa ⤳ ?σb |- _] =>
+        apply hoare_reductions_implies_pair_reduction with (M:=Mc)(σ2:=σb);
+        auto
+      end
+    end.
+
+  Lemma internal_MyModule1_is_take :
+    forall M σ, internal_step MyModule1 M σ ->
+           forall M', MyModule1 ⋄ M ≜ M' ->
+                 exists x y mySecret s, contn_is (s_meth x y take (update scr mySecret empty) ;; s) σ /\
+                                 classOf y σ Safe /\
+                                 (M' ∙ σ ⊢ (e_var mySecret ⩵ (e_acc_f (e_var y) secret)) ↪ v_true \/
+                                  M' ∙ σ ⊢ (e_var mySecret ⩵ (e_acc_f (e_var y) secret)) ↪ v_false).
+  Proof.
+  Admitted.
+
+  Parameter take_correct_secret_unchanged_heap :
+    forall M M', MyModule1 ⋄ M ≜ M' ->
+            forall σ x y mySecret s α , MyModule1 ⦂ M ⦿
+                                             {pre: fun σ => contn_is ((s_meth x y take (update scr mySecret empty) ;; s)) σ /\
+                                                         ⟦ y ↦ (v_addr α) ⟧ ∈ σ /\
+                                                         classOf y σ Safe /\
+                                                         M' ∙ σ ⊢ (e_var mySecret ⩵ (e_acc_f (e_var y) secret)) ↪ v_true}
+                                             σ
+                                             {post: fun σ' => M' ∙ σ' ⊢ (e_acc_f (e_var y) secret) ↪ v_null}.
+
+  Parameter take_incorrect_secret_unchanged_heap :
+    forall M M', MyModule1 ⋄ M ≜ M' ->
+            forall σ x y mySecret s, MyModule1 ⦂ M ⦿
+                                          {pre: fun σ => contn_is ((s_meth x y take (update scr mySecret empty) ;; s)) σ /\
+                                                      classOf y σ Safe /\
+                                                      M' ∙ σ ⊢ (e_var mySecret ⩵ (e_acc_f (e_var y) secret)) ↪ v_false}
+                                          σ
+                                          {post: heapUnchanged σ}.
+  
+  Definition HolisticSpec := (∀x∙ (∀x∙(((a_class (a♢1) Safe)
+                                        ∧
+                                        ((ex_acc_f (e♢1) secret) ⩶ (e♢0))
+                                        ∧
+                                        ((ex_acc_f (e♢1) treasure) ⩶̸ (ex_null))
+                                         ∧
+                                         (a_will ((ex_acc_f (e♢1) treasure) ⩶ (ex_null))))
+                                           ⟶
+                                           (a_will (∃x∙ (((a♢0) external)
+                                                         ∧
+                                                         ((a♢0) access (a♢1))))
+                                            ∨
+                                            (∃x∙ (((a♢0) external)
+                                                  ∧
+                                                  ((a♢0) access (a♢1))))
+                             )))).
+
+  Theorem safe_example :
+    MyModule1 ⊨m HolisticSpec.
+  Proof.
+    unfold mdl_sat;
+      intros;
+      destruct_exists_loo.
+    unfold HolisticSpec;
+      a_intros.
+    a_prop.
+    inversion H5;
+      subst.
+    let σ := fresh "σ" in
+    destruct (pair_reduction_change MyModule1 M' (χ, ϕ :: nil) σ')
+      with (P := fun (M1 M2 : mdl)(σ : config) =>
+                   M1 ⦂ M2 ◎ (χ, ϕ :: nil) … σ ⊨ (ex_acc_f (e_ α) treasure ⩶̸ (ex_null)))
+      as [σ];
+      auto.
+    + eapply sat_head_exp; eauto.
+      eapply sat_initial_exp; eauto.
+
+    + intros Hcontra.
+      inversion H15; subst.
+      inversion Hcontra;
+        subst.
+      link_unique_auto.
+      repeat match goal with
+             | [H : is_exp ?e ?e' |- _] =>
+               inversion H;
+                 subst;
+                 clear H
+             end.
+      inversion H20; subst.
+      inversion H18; subst.
+      eval_rewrite.
+      crush.
+
+    + destruct_exists_loo;
+        andDestruct.
+      destruct (pair_reduction_inversion_hoare MyModule1 M' σ σ1); auto.
+      * apply external_step_leaves_internal_field_unchanged
+          with
+            (σ':=σ1)
+          in Ha2;
+          auto.
+        -- contradiction Hb0; auto.
+        -- apply internal_class_implies_internal with (σ0:=σ0)(σ:=(χ, ϕ :: ψ))(C:=Safe); auto.
+           exists SafeDef1; unfold MyModule1.
+           repeat map_rewrite.
+      * apply internal_MyModule1_is_take with (M':=M) in H8; auto;
+          repeat destruct_exists_loo;
+          andDestruct.
+        destruct Hb1.
+        -- destruct Ha;
+             subst;
+             [right|left].
+           ++ assert (Hex : external_self MyModule1 M' (χ, ϕ :: ψ));
+                [eapply external_self_head1, pair_reductions_external_self1; eauto
+                |unfold external_self, is_external in Hex;
+                 repeat destruct_exists_loo;
+                 andDestruct].
+              apply sat_ex_x with (α:=α1)(o:=o1);
+                auto; simpl; a_prop.
+              ** eapply sat_extrn; eauto.
+              ** inversion Ha3;
+                   subst;
+                   simpl in *;
+                   repeat simpl_crush.
+                 eapply sat_access3 with (x:=x2); eauto with loo_db.
+                 --- admit. (* α is the only changed object in the heap *)
+                 --- apply in_stmts_1, in_meth_3; exists scr; repeat map_rewrite.
+           ++ apply sat_will with (ϕ:=ϕ)(ψ:=ψ)(χ:=χ)(σ':=σ);
+                auto.
+              assert (Hex : external_self MyModule1 M' σ);
+                [eapply pair_reductions_external_self2; eauto
+                |unfold external_self, is_external in Hex;
+                 repeat destruct_exists_loo;
+                 andDestruct].
+              apply sat_ex_x with (α:=α1)(o:=o1);
+                auto; simpl; a_prop.
+              ** eapply sat_extrn; eauto.
+              ** inversion Ha3;
+                   subst;
+                   simpl in *;
+                   destruct σ as [χ' ψ'];
+                   simpl in *;
+                   subst;
+                   repeat simpl_crush.
+                 eapply sat_access3 with (x:=x2); eauto with loo_db.
+                 --- admit.
+                 --- apply in_stmts_1, in_meth_3; exists scr; repeat map_rewrite.
+
+        -- contradiction (fieldChange_not_heapUnchanged MyModule1 M' (χ, ϕ :: nil) σ α treasure (ex_null))
+             with (σ':=σ1); auto.
+           ++ apply ht_pr;
+                intros.
+              unique_reduction_auto.
+              apply not_neq_implies_eq;
+                auto.
+           ++ eapply hoare_triple_pr_inversion with (M1:=MyModule1)(M2:=M')(σ:=σ);
+                auto.
+              apply take_incorrect_secret_unchanged_heap; simpl; eauto.
+              simpl.
+              split; eauto.
+  Admitted.
+End SafeExample.
+                 
